wip

clight_examples/xorlist/xorlist.v
@@ -115,6 +115,9 @@ Definition _t'5 : ident := 132%positive.
 Definition _t'6 : ident := 133%positive.
 Definition _t'7 : ident := 134%positive.
 Definition _t'8 : ident := 135%positive.
+Definition _t'9 : ident := 136%positive.
+Definition _t'10 : ident := 137%positive.
+Definition _t'11 : ident := 138%positive.
 
 Definition f_encrypt := {|
   fn_return := tlong;
@@ -122,13 +125,13 @@ Definition f_encrypt := {|
   fn_params := ((_prev, (tptr (Tstruct __Node noattr))) ::
                 (_next, (tptr (Tstruct __Node noattr))) :: nil);
   fn_vars := nil;
-  fn_temps := nil;
+  fn_temps := ((_t'9, tlong) :: (_t'10, tlong) :: nil);
   fn_body :=
-(Sreturn (Some (Ebinop Oxor
-                 (Ecast (Etempvar _prev (tptr (Tstruct __Node noattr)))
-                   tlong)
-                 (Ecast (Etempvar _next (tptr (Tstruct __Node noattr)))
-                   tlong) tlong)))
+(Ssequence
+   (Sbuiltin (Some _t'9) EF_capture (Tcons (tptr (Tstruct __Node noattr)) Tnil) ((Etempvar _prev (tptr (Tstruct __Node noattr))) :: nil))
+   (Ssequence
+      (Sbuiltin (Some _t'10) EF_capture (Tcons (tptr (Tstruct __Node noattr)) Tnil) ((Etempvar _next (tptr (Tstruct __Node noattr))) :: nil))
+      (Sreturn (Some (Ebinop Oxor (Etempvar _t'9 tlong) (Etempvar _t'10 tlong) tlong)))))
 |}.
 
 Definition f_decrypt := {|
@@ -137,12 +140,11 @@ Definition f_decrypt := {|
   fn_params := ((_key, tlong) :: (_ptr, (tptr (Tstruct __Node noattr))) ::
                 nil);
   fn_vars := nil;
-  fn_temps := nil;
+  fn_temps := ((_t'11, tlong) :: nil);
   fn_body :=
-(Sreturn (Some (Ecast
-                 (Ebinop Oxor (Etempvar _key tlong)
-                   (Ecast (Etempvar _ptr (tptr (Tstruct __Node noattr)))
-                     tlong) tlong) (tptr (Tstruct __Node noattr)))))
+  (Ssequence
+    (Sbuiltin (Some _t'11) EF_capture (Tcons (tptr (Tstruct __Node noattr)) Tnil) ((Etempvar _ptr (tptr (Tstruct __Node noattr))) :: nil))
+    (Sreturn (Some (Ecast (Ebinop Oxor (Etempvar _key tlong) (Etempvar _t'11 tlong) tlong) (tptr (Tstruct __Node noattr))))))
 |}.
 
 Definition f_add := {|
