clight_examples/xorlist/xorlist01proof.v
@@ -1,73 +1,197 @@
-(* Require Import Coqlib. *)
-(* Require Import Any. *)
-(* Require Import Skeleton. *)
-(* Require Import PCM. *)
-(* Require Import ModSem. *)
-(* Require Import SimModSem. *)
-(* Require Import HoareDef. *)
-(* Require Import STB. *)
-(* Require Import HTactics ProofMode. *)
-(* Require Import ConvC2ITree. *)
-(* Require Import Clight_Mem1. *)
-(* Require Import ClightProofs. *)
-(* Require Import ClightPreambles. *)
-(* Require Import csyntax. *)
 Require Import Coqlib.
-Require Import ImpPrelude.
+Require Import Any.
 Require Import STS.
 Require Import Behavior.
 Require Import ModSem.
 Require Import Skeleton.
+Require Import SimModSem.
 Require Import PCM.
 Require Import HoareDef.
-Require Import ProofMode.
 Require Import STB.
 Require Import HTactics ProofMode.
-Require Import SimModSem.
-Require Import Coq.Sorting.Sorted.
-Require Import ClightProofs.
-Require Import csyntax.
-Require Import ConvC2ITree.
-Require Import Clight_Mem1.
-Require Import ClightPreambles.
+Require Import HSim IProofMode.
+Require Import ClightDmgen.
+Require Import ClightDmMem1.
+Require Import xorlist.
 Require Import xorlist0.
 Require Import xorlist1.
+Require Import CTactics.
+(* Require Import ClightProofs.
+Require Import csyntax.
+Require Import ClightPreambles. *)
 
-(* From compcertip Require Import Clightdefs. *)
+From Coq Require Import Program.
+From compcertip Require Import Clightdefs.
 
-Section XorProof.
 
-  Import CTypeNotation CExpNotation CStmtNotation.
+Section LEMMA.
+
+  Lemma f_bind_ret_r E R A (s : A -> itree E R)
+    : (fun a => ` x : R <- (s a);; Ret x) = s.
+  Proof. apply func_ext. i. apply bind_ret_r. Qed.
+
+End LEMMA.
+
+Section PROOF.
+
+  (* Import CTypeNotation CExpNotation CStmtNotation.
   Local Open Scope cexp_scope.
   Local Open Scope cstmt_scope.
-  Local Open Scope ctypes_scope.
+  Local Open Scope ctypes_scope. *)
   
   (* Context `{CONF: EMSConfig}. *)
-  Context `{Σ : GRA.t}.
-  Context `{H : @GRA.inG Clight_Mem1.memRA Σ}.
-  Context `{H1 : @GRA.inG Clight_Mem1.memRACAP Σ}.
+  Context `{@GRA.inG memcntRA Σ}.
+  Context `{@GRA.inG memphyRA Σ}.
+  Context `{@GRA.inG memhdRA Σ}.
+  Context `{@GRA.inG memidRA Σ}.
   
   Variable GlobalStb : Sk.t -> gname -> option fspec.
-  Hypothesis STBINCL : forall sk, stb_incl (to_stb xorlist1.xorStb) (GlobalStb sk).
-  Hypothesis MEMINCL : forall sk, stb_incl (to_stb Clight_Mem1.MemStb) (GlobalStb sk).
+  Hypothesis STBINCL : forall sk, stb_incl (to_stb xorStb) (GlobalStb sk).
+  Hypothesis MEMINCL : forall sk, stb_incl (to_stb MemStb) (GlobalStb sk).
+
+  Opaque get_sk.
+  Opaque prog_comp_env.
 
   Definition wf : _ -> Any.t * Any.t -> Prop :=
     @mk_wf
       _
       unit
-      (fun _ st_src st_tgt => True)%I.
-
-  Lemma sim_encrypt (sk: alist string Sk.gdef) :
-    sim_fnsem wf top2
-      ("encrypt",
-        fun_to_tgt (SModSem.mn (SMod.get_modsem Sxor sk)) (GlobalStb sk)
-                   {| fsb_fspec := encrypt_spec; fsb_body := λ _ : option string * Any.t, triggerNB |})
-      ("encrypt", cfunU xorlist0.encrypt_body).
+      (fun _ st_src st_tgt => ⌜True⌝)%I.
+  
+  (* Theorem correct : refines2 [xorlist0.xor] [xorlist1.xor GlobalStb].
   Proof.
-  Opaque Maps.PTree.set.
-  Opaque Maps.PTree.get.
-  Opaque decomp_stmt.
-    init. harg. destruct x. destruct p as [[v1 v2] mvl1]. mDesAll. des.
+    eapply adequacy_local2. econs; ss.
+    i. econstructor 1 with (wf := wf) (le := top2); et; ss; cycle 1.
+    { eexists. econs. apply to_semantic. iIntros. et. }
+    (* each functions has simulation relation *)
+    econs; cycle 1.
+    econs; cycle 1.
+    econs; cycle 1.
+    econs; cycle 1.
+    econs; et.
+    all: rewrite f_bind_ret_r.
+    - apply sim_search.
+    - apply sim_delete.
+    - apply sim_add.
+    - apply sim_decrypt.
+    - apply sim_encrypt.
+  Qed. *)
+  Arguments alist_add /.
+  Arguments ccallU /.
+
+  Let ce := map (fun '(id, p) => (string_of_ident id, p)) (Maps.PTree.elements (prog_comp_env prog)).
+
+  Lemma val_multimap v b ofs : (v ⊸ (b, ofs)) -∗ ⌜exists i, v = Vptrofs i \/ exists b ofs, v = Vptr b ofs⌝.
+  Proof.
+    iIntros "A". destruct v; ss; des_ifs_safe.
+    - unfold Vptrofs. des_ifs_safe. iPureIntro. exists (Ptrofs.of_int64 i).
+      rewrite Ptrofs.to_int64_of_int64; et.
+    - iDestruct "A" as "[% %]". iPureIntro. des. clarify. et.
+    Unshelve. et. 
+  Qed.
+
+  Lemma val_exists i b ofs q0 z t a : Vptrofs i ⊸ (b, ofs) ** b ↱q0# (z, t, a) 
+    -∗ b ↱q0# (z, t, Some (Ptrofs.unsigned i)).
+  Proof. Admitted.
+
+  Lemma sim_encrypt (sk: Sk.t) :
+    sim_fnsem wf top2
+      ("encrypt", fun_to_tgt "xorlist" (GlobalStb sk) (mk_pure encrypt_spec))
+      ("encrypt", cfunU (decomp_func sk ce f_encrypt)).
+  Proof.
+    Opaque repr_to.
+    Opaque allocated_with.
+    Opaque points_to.
+    Opaque Maps.PTree.set.
+    Opaque Maps.PTree.get.
+    econs; ss. red.
+    apply isim_fun_to_tgt; auto. i; ss.
+    unfold decomp_func, function_entry_c. ss.
+    iIntros "[INV PRE]". des_ifs_safe. ss.
+    iDestruct "PRE" as "[PRE %]".
+    iDestruct "PRE" as (ofs1 ofs2 opt1 opt2) "[[[[% PTR1] ARG1] PTR2] ARG2]".
+    ss. clarify. hred_r. iApply isim_tau_tgt. hred_r. iApply isim_tau_tgt.
+    ss. hred_r. des_ifs_safe.
+    iApply isim_apc. iExists (Some (2 : Ord.t)).
+    iPoseProof (val_multimap with "PTR1") as "%".
+    iPoseProof (val_multimap with "PTR2") as "%".
+    des.
+    - unfold Vptrofs in *; des_ifs_safe. hred_r.
+      iApply isim_call_pure.
+      { eapply fn_has_spec_in_stb.
+        { eapply MEMINCL. stb_tac. ss. }
+        { oauto. }
+        { ss. } }
+      { oauto. }
+      iSplitL "INV".
+      { iSplitL "INV"; auto. ss.
+        iSplits; ss. instantiate (1:=True%I); et. }
+      iIntros (st_src0 st_tgt0 ret_src ret_tgt) "[INV POST]".
+      ss. iDestruct "POST" as "[% %]". ss. clarify.
+      hred_r. iApply isim_tau_tgt. hred_r. iApply isim_tau_tgt.
+      hred_r. iApply isim_tau_tgt. ss. hred_r.
+      iApply isim_call_pure.
+      { eapply fn_has_spec_in_stb.
+        { eapply MEMINCL. stb_tac. ss. }
+        { oauto. }
+        { ss. } }
+      { oauto. }
+      iSplitL "INV".
+      { iSplitL "INV"; auto. ss.
+        iSplits; ss. instantiate (1:=True%I); et. }
+      iIntros (st_src1 st_tgt1 ret_src ret_tgt) "[INV POST]".
+      ss. iDestruct "POST" as "[% %]". ss. clarify.
+      hred_r. iApply isim_tau_tgt. hred_r. iApply isim_tau_tgt. ss.
+      hred_r.
+      unfold ClightDmExprgen.sem_xor_c, ClightDmExprgen.sem_binarith_c, ClightDmExprgen.sem_cast_c.
+      ss. des_ifs_safe. hred_r. hred_l. iApply isim_choose_src. iExists _.
+      iApply isim_ret. iSplits; ss.
+      iSplitR "ARG2". 
+      iSplitR "ARG1".
+      {  } 
+
+
+
+      
+      iSplitL "-"; auto.
+      acatch. { apply MEMINCL. stb_tac. auto. } steps.
+      hcall (fun vret => ⌜vret = (Vlong (Ptrofs.to_int64 i0))↑⌝%I) _ with "".
+      { iModIntro. iSplits; ss. instantiate (1:=True%I). et. }
+      { oauto. }
+      mDesAll. des. subst. steps.
+      acatch. { apply MEMINCL. stb_tac. auto. }
+      steps.
+      hcall (fun vret => ⌜vret = (Vlong (Ptrofs.to_int64 i))↑⌝%I) _ with "".
+      { iModIntro. iSplits; ss. instantiate (1:=True%I). et. }
+      { oauto. }
+      mDesAll. des. subst. steps.
+      unfold ClightDmExprgen.sem_xor_c, ClightDmExprgen.sem_binarith_c, ClightDmExprgen.sem_cast_c.
+      steps. astop. steps. force_l. eexists. steps. hret tt; ss.
+      iModIntro. iSplits; ss.
+      iSplitR "A A1". iSplitR "A3 A2".
+      all: cycle 1.
+      { iApply val_exists. iFrame. }
+      { iApply val_exists. iFrame. }
+      iPureIntro. repeat f_equal. admit.
+    - unfold Vptrofs in *; des_ifs_safe. steps.
+      acatch. { apply MEMINCL. stb_tac. auto. } steps.
+      hcall _ _ with "".
+      { iModIntro. iSplits; ss.
+        { unfold capture_resource. iPureIntro. eexists _, _, _.
+          et. }
+       instantiate (1:=True%I). et. }
+      { oauto. }
+      mDesAll. des. subst. steps.
+
+     admit.
+    - unfold Vptrofs in *; des_ifs_safe. steps. admit.
+    - steps. admit.
+    mDesAll.
+    des_ifs; ss; des_ifs_safe; mDesAll; try solve [inv PURE]; steps.
+    - 
+    unfold alist_add. ss. alist_remove. ss.
+    repeat (rewrite decomp_seq); steps.
+    destruct build_composite_env'. steps. 
     steps. unfold function_entry_c. steps. resolve_seq. 
     unfold is_valid_ptr in ACC. 
     destruct v1;destruct v2;mDesAll;ss;steps.
@@ -247,23 +371,19 @@ fix set (A : Type) (i : positive) (v : A) (m : PTree.t A) {struct i} : PTree.t A
  
   Theorem correct : refines2 [xorlist0.xor] [xorlist1.xor GlobalStb].
   Proof.
-    eapply SimModSem.adequacy_local2. econs.
-    2:{ simpl. reflexivity. }
-    i. econstructor 1 with (wf := wf) (le := top2).
-    (* kripke order is preorder *)
-    { econs. unfold Reflexive. auto. unfold Transitive. auto. }
-    (* two module have same name *)
-    2:{ simpl. auto. }
-    (* if initial resource is well formed, initial condition is satisfied *)
-    2:{ exists tt. econs. apply to_semantic. iIntros. auto. }
+    eapply adequacy_local2. econs; ss.
+    i. econstructor 1 with (wf := wf) (le := top2); et; ss; cycle 1.
+    { eexists. econs. apply to_semantic. iIntros. et. }
     (* each functions has simulation relation *)
-    econs;cycle 1.
-    econs;cycle 1.
-    econs;cycle 1.
-    econs;cycle 1.
-    econs.
+    econs; cycle 1.
+    econs; cycle 1.
+    econs; cycle 1.
+    econs; cycle 1.
+    econs; et.
+    all: rewrite f_bind_ret_r.
+    - apply sim_search.
     - apply sim_delete.
-    - apply sim_insert.
+    - apply sim_add.
     - apply sim_decrypt.
     - apply sim_encrypt.
   Qed.
