clight_examples/xorlist/xorlist0.v
@@ -5,4 +5,4 @@ Require Import Any.
 Require Import ClightDmgen.
 Require Import xorlist.
 
-Definition xor : Mod.t := get_mod composites global_definitions Logic.I "xorlist".
+Definition xor : Mod.t := get_mod prog "xorlist".
